lua.v
@@ -70,7 +70,7 @@ Fixpoint Lua2Lir (e : LE) : IRE :=
   | LEFun var body =>
       IREBox TgFun (IREFun var
          (IRELet var IRTStar (IREVar var) (Lua2Lir body)))
-  | LEApp e1 e2 => IREFunApp (IREUnbox TgFun (Lua2Lir e1)) (Lua2Lir e2)
+  | LEApp e1 e2 => IREApp (IREUnbox TgFun (Lua2Lir e1)) (Lua2Lir e2)
   end.
 
 
